src/Stackability.v
@@ -6,7 +6,7 @@ From Celsius Require Export PartialMonotonicity Reachability Wellformedness.
 Require Import ssreflect ssrbool Psatz List.
 Import ListNotations.
 Open Scope nat_scope.
-Implicit Type (σ: Store) (ρ ω: Env) (l: Loc) (L: LocSet).
+Implicit Type (σ: Store) (ρ ω: Env) (l: Loc) (L: LocSet) (el: list Expr).
 Global Hint Resolve eM_warm_monotone: stk.
 
 
@@ -49,51 +49,78 @@ Qed.
 Global Hint Resolve stk_trans: stk.
 
 (** Assignment *)
-Lemma stk_assign : forall σ l C ω ω',
+Lemma stk_assign : forall σ l C ω f v,
     getObj σ l = Some (C, ω) ->
-    length ω <= length ω' ->
-    σ ≪ [l ↦ (C, ω')]σ.
+    σ ≪ [l ↦ (C, [f ↦ v]ω)]σ.
 Proof.
   autounfold with stk notations; steps.
   updates; eauto.
 Qed.
-Global Hint Resolve stk_assign: stk.
+Local Hint Resolve stk_assign: stk.
+
+Lemma stk_assign_new : forall σ l C ω v,
+    getObj σ l = Some (C, ω) ->
+    σ ≪ [l ↦ (C, ω++[v])]σ.
+Proof.
+  autounfold with stk notations; steps.
+  updates; eauto.
+Qed.
+Local Hint Resolve stk_assign_new: stk.
+
 
 
 (** ** Main stackability theorem *)
 (** Here we show the main result. We proceed by induction, enriching the goal with partial monotonicity and compatibility.Stackability is not maintained throughout the initialization of a new object, as its fields are being initialized. For the proof, we use a custom predicate [Pin] : the stores grows and the number of initialized fields grows too. Doing this, when we reach the end of initialization, we get a store with all initialized fields for the new object  *)
 
 Theorem stk_theorem :
-  forall e σ σ' ρ ψ v,
-    ⟦e⟧ (σ, ρ, ψ) --> (v, σ') -> σ ≪ σ'.
-Proof with (updates; eauto 3 with stk pM updates lia ).
-  intros.
-  induction H using evalP_ind2 with
-    (Pl := fun _ σ _ _ _ σ' _ => σ ≪ σ')
-    (Pin := fun C fls I _ σ σ' _   =>
-              forall ω, getObj σ I = Some (C, ω) ->
-                σ ≪ σ' /\ (exists ω', getObj σ' I = Some (C, ω') /\ (length fls + length ω = length ω')));
-    unfold assign, assign_new in * ; eval_dom;
-    try solve [steps; eauto with stk pM]...
-  - rewrite getObj_last in IHevalP0.
-    move /(_ [] eq_refl): IHevalP0. steps ...
+  (forall e σ ρ ψ v σ',
+      ⟦e⟧ (σ, ρ, ψ) --> (v, σ') -> σ ≪ σ') /\
+    (forall el σ ρ ψ vl σ',
+        ⟦el⟧ (σ, ρ, ψ) --> (vl, σ') -> σ ≪ σ') /\
+    (forall C flds I ρ σ σ',
+        initP C flds I ρ σ σ' ->
+        (forall ω, getObj σ I = Some (C, ω) ->
+             σ ≪ σ' /\ (exists ω', getObj σ' I = Some (C, ω') /\ (length flds + length ω = length ω')))).
+
+Proof with (updates; eauto 4 with stk pM lia ).
+
+  apply evalP_multi_ind;
+    unfold assign, assign_new; simpl; intros;
+    eval_dom; ss_trans;
+    try solve [intuition (eauto 3 with stk pM lia)].
+
+  - eapply stk_trans...
+  - rewrite getObj_last in IH__init.
+    move /(_ [] eq_refl): IH__init. steps ...
     eapply stk_trans with σ1; try eapply pM_trans with (σ1 ++ [(C, [])])...
     move => l Hl.
     move /(_ l Hl): H1 => H1. steps ...
     destruct_eq (l = dom σ1); steps; [left |] ...
     repeat eexists ...
   - steps ; pM_trans ...
-    eapply stk_trans with ([v1 ↦ (c, [x ↦ v2] (e))] (σ2)) ...
-    eapply stk_trans with σ2 ...
-    eapply stk_trans with σ2 ...
-  - intros.
-    repeat destruct_match => //.
-    invert_constructor_equalities; subst...
-    lets [?ω [ ]]: eM_theorem H H2.
-    rewrite getObj_update_same in IHevalP0 ...
-    cross_rewrites.
-    move /(_ _ eq_refl): IHevalP0. steps ...
+    + eapply stk_trans with ([v1 ↦ (c, [x ↦ v2] (e))] (σ2)) ...
+      eapply stk_trans with σ2 ...
+    + eapply stk_trans with σ2 ...
+  - lets [?ω [ ]]: eM_theorem_expr H__e H.
+    rewrite H2 in H__assign; inverts H__assign.
+    rewrite getObj_update_same in IH__flds; eauto with updates ...
+    move /(_ _ eq_refl): IH__flds; intros; flatten; updates.
+    split...
     eapply stk_trans with ([I ↦ (C, ω0 ++ [v])] (σ1)) ...
-    eapply stk_trans with σ1 ...
 Qed.
-Global Hint Resolve stk_theorem: stk.
+
+Corollary stk_theorem_expr :
+  forall e σ ρ ψ v σ',
+    ⟦e⟧ (σ, ρ, ψ) --> (v, σ') -> σ ≪ σ'.
+Proof.
+  apply stk_theorem.
+Qed.
+Global Hint Resolve stk_theorem_expr: stk.
+
+Corollary stk_theorem_list :
+    forall el σ ρ ψ vl σ',
+      ⟦el⟧ (σ, ρ, ψ) --> (vl, σ') -> σ ≪ σ'.
+Proof.
+  apply stk_theorem.
+Qed.
+Global Hint Resolve stk_theorem_list: stk.
